theories/auth_excl.v
@@ -1,0 +1,54 @@
+From iris.heap_lang Require Export lang.
+From iris.proofmode Require Import tactics.
+From iris.algebra Require Import excl auth.
+From iris.base_logic.lib Require Import auth.
+Set Default Proof Using "Type".
+
+Definition exclUR (A : Type) : ucmraT :=
+  optionUR (exclR (leibnizC A)).
+
+Class auth_exclG (A : Type) (Σ :gFunctors) :=
+  AuthExclG {
+      exclG_authG :> authG Σ (exclUR A);
+    }.
+
+Definition auth_exclΣ (A : Type) : gFunctors :=
+  #[GFunctor (authR (exclUR A))].
+
+Instance subG_auth_exclG (A : Type) {Σ} :
+  subG (auth_exclΣ A) Σ → (auth_exclG A) Σ.
+Proof. solve_inG. Qed.
+
+Definition to_auth_excl {A : Type} (a : A) : exclUR A :=
+  Excl' (a: leibnizC A).
+
+Section auth_excl.
+  Context `{!auth_exclG A Σ} (N : namespace).
+
+  Lemma excl_eq γ x y :
+    own γ (● to_auth_excl y) -∗ own γ (◯  to_auth_excl x) -∗ ⌜x = y⌝%I.
+  Proof.
+    iIntros "Hauth Hfrag".
+    iDestruct (own_valid_2 with "Hauth Hfrag") as %Hvalid.
+    apply auth_valid_discrete_2 in Hvalid.
+    destruct Hvalid as [Hincl _].
+    apply Excl_included in Hincl.
+    unfold to_auth_excl.
+    rewrite Hincl.
+    iFrame.
+    eauto.
+  Qed.
+  
+  Lemma excl_update γ x y z :
+    own γ (● to_auth_excl y) -∗ own γ (◯  to_auth_excl x) -∗ |==> own γ (● to_auth_excl z) ∗ own γ (◯  to_auth_excl z).
+  Proof.
+    iIntros "Hauth Hfrag".
+    iDestruct (own_update_2 with "Hauth Hfrag") as "H".
+    { eapply (auth_update _ _ (to_auth_excl z) (to_auth_excl z)).
+      eapply option_local_update.
+      eapply exclusive_local_update. done. }
+    rewrite own_op.
+    done.
+  Qed.
+
+End auth_excl.
